cfrontend/Csharpminor.v
@@ -327,6 +327,7 @@ Section EVAL_EXPR.
 
 Variable e: env.
 Variable le: temp_env.
+Variable cp: compartment.
 Variable m: mem.
 (* JT: TODO: Might probably need to add a compartment variable to this section *)
 
@@ -349,7 +350,7 @@ Inductive eval_expr: expr -> val -> Prop :=
       eval_expr a2 v2 ->
       eval_binop op v1 v2 m = Some v ->
       eval_expr (Ebinop op a1 a2) v
-  | eval_Eload: forall chunk a v1 cp v,
+  | eval_Eload: forall chunk a v1 v,
       eval_expr a v1 ->
       Mem.loadv chunk m v1 cp = Some v ->
       eval_expr (Eload chunk a) v.
@@ -371,6 +372,7 @@ End EVAL_EXPR.
 
 (** One step of execution *)
 
+(* FIXME: replaced a number of arbitrarily quantified cps with comp_of. *)
 Inductive step: state -> trace -> state -> Prop :=
 
   | step_skip_seq: forall f s k e le m,
@@ -379,27 +381,27 @@ Inductive step: state -> trace -> state -> Prop :=
   | step_skip_block: forall f k e le m,
       step (State f Sskip (Kblock k) e le m)
         E0 (State f Sskip k e le m)
-  | step_skip_call: forall f k e le m cp m',
+  | step_skip_call: forall f k e le m m',
       is_call_cont k ->
-      Mem.free_list m (blocks_of_env e) cp = Some m' ->
+      Mem.free_list m (blocks_of_env e) (comp_of f) = Some m' ->
       step (State f Sskip k e le m)
         E0 (Returnstate Vundef k m')
 
   | step_set: forall f id a k e le m v,
-      eval_expr e le m a v ->
+      eval_expr e le (comp_of f) m a v ->
       step (State f (Sset id a) k e le m)
         E0 (State f Sskip k e (PTree.set id v le) m)
 
-  | step_store: forall f chunk addr a k e le m vaddr v cp m',
-      eval_expr e le m addr vaddr ->
-      eval_expr e le m a v ->
-      Mem.storev chunk m vaddr v cp = Some m' ->
+  | step_store: forall f chunk addr a k e le m vaddr v m',
+      eval_expr e le (comp_of f) m addr vaddr ->
+      eval_expr e le (comp_of f) m a v ->
+      Mem.storev chunk m vaddr v (comp_of f)  = Some m' ->
       step (State f (Sstore chunk addr a) k e le m)
         E0 (State f Sskip k e le m')
 
   | step_call: forall f optid sig a bl k e le m vf vargs fd,
-      eval_expr e le m a vf ->
-      eval_exprlist e le m bl vargs ->
+      eval_expr e le (comp_of f) m a vf ->
+      eval_exprlist e le (comp_of f) m bl vargs ->
       Genv.find_funct ge vf = Some fd ->
       funsig fd = sig ->
       forall (ALLOWED: Policy.allowed_call pol f.(fn_comp) fd),
@@ -407,7 +409,7 @@ Inductive step: state -> trace -> state -> Prop :=
         E0 (Callstate fd vargs (Kcall optid f e le k) m)
 
   | step_builtin: forall f optid ef bl k e le m vargs t vres m',
-      eval_exprlist e le m bl vargs ->
+      eval_exprlist e le (comp_of f) m bl vargs ->
       external_call ef ge f.(fn_comp) vargs m t vres m' ->
       step (State f (Sbuiltin optid ef bl) k e le m)
          t (State f Sskip k e (Cminor.set_optvar optid vres le) m')
@@ -417,7 +419,7 @@ Inductive step: state -> trace -> state -> Prop :=
         E0 (State f s1 (Kseq s2 k) e le m)
 
   | step_ifthenelse: forall f a s1 s2 k e le m v b,
-      eval_expr e le m a v ->
+      eval_expr e le (comp_of f) m a v ->
       Val.bool_of_val v b ->
       step (State f (Sifthenelse a s1 s2) k e le m)
         E0 (State f (if b then s1 else s2) k e le m)
@@ -441,18 +443,18 @@ Inductive step: state -> trace -> state -> Prop :=
         E0 (State f (Sexit n) k e le m)
 
   | step_switch: forall f islong a cases k e le m v n,
-      eval_expr e le m a v ->
+      eval_expr e le (comp_of f) m a v ->
       switch_argument islong v n ->
       step (State f (Sswitch islong a cases) k e le m)
         E0 (State f (seq_of_lbl_stmt (select_switch n cases)) k e le m)
 
-  | step_return_0: forall f k e le m cp m',
-      Mem.free_list m (blocks_of_env e) cp = Some m' ->
+  | step_return_0: forall f k e le m m',
+      Mem.free_list m (blocks_of_env e) (comp_of f)  = Some m' ->
       step (State f (Sreturn None) k e le m)
         E0 (Returnstate Vundef (call_cont k) m')
-  | step_return_1: forall f a k e le m v cp m',
-      eval_expr e le m a v ->
-      Mem.free_list m (blocks_of_env e) cp = Some m' ->
+  | step_return_1: forall f a k e le m v m',
+      eval_expr e le (comp_of f) m a v ->
+      Mem.free_list m (blocks_of_env e) (comp_of f) = Some m' ->
       step (State f (Sreturn (Some a)) k e le m)
         E0 (Returnstate v (call_cont k) m')
   | step_label: forall f lbl s k e le m,
