cfrontend/SimplExprspec.v
@@ -64,16 +64,16 @@ Inductive tr_expr: temp_env -> destination -> Csyntax.expr -> list statement -> 
       tr_expr le For_effects (Csyntax.Eval v ty) nil any tmp
   | tr_val_value: forall le v ty a tmp,
       typeof a = ty ->
-      (forall tge e le' m,
+      (forall tge e le' cp m,
          (forall id, In id tmp -> le'!id = le!id) ->
-         eval_expr tge e le' m a v) ->
+         eval_expr tge e le' cp m a v) ->
       tr_expr le For_val (Csyntax.Eval v ty)
                            nil a tmp
   | tr_val_set: forall le sd v ty a any tmp,
       typeof a = ty ->
-      (forall tge e le' m,
+      (forall tge e le' cp m,
          (forall id, In id tmp -> le'!id = le!id) ->
-         eval_expr tge e le' m a v) ->
+         eval_expr tge e le' cp m a v) ->
       tr_expr le (For_set sd) (Csyntax.Eval v ty)
                    (do_set sd a) any tmp
   | tr_sizeof: forall le dst ty' ty tmp,
@@ -367,17 +367,20 @@ Qed.
   [tr_expr], the Cminor expression must not depend on memory,
   while in the case of [tr_top] it can depend on the current memory
   state. *)
+(* NOTE: If there are no memory dependencies, compartments have no
+   effect on evaluation either. *)
 
 Section TR_TOP.
 
 Variable ge: genv.
 Variable e: env.
 Variable le: temp_env.
+Variable cp: compartment.
 Variable m: mem.
 
 Inductive tr_top: destination -> Csyntax.expr -> list statement -> expr -> list ident -> Prop :=
   | tr_top_val_val: forall v ty a tmp,
-      typeof a = ty -> eval_expr ge e le m a v ->
+      typeof a = ty -> eval_expr ge e le cp m a v ->
       tr_top For_val (Csyntax.Eval v ty) nil a tmp
   | tr_top_base: forall dst r sl a tmp,
       tr_expr le dst r sl a tmp ->
@@ -389,17 +392,17 @@ End TR_TOP.
 
 Inductive tr_expression: Csyntax.expr -> statement -> expr -> Prop :=
   | tr_expression_intro: forall r sl a tmps,
-      (forall ge e le m, tr_top ge e le m For_val r sl a tmps) ->
+      (forall ge e le cp m, tr_top ge e le cp m For_val r sl a tmps) ->
       tr_expression r (makeseq sl) a.
 
 Inductive tr_expr_stmt: Csyntax.expr -> statement -> Prop :=
   | tr_expr_stmt_intro: forall r sl a tmps,
-      (forall ge e le m, tr_top ge e le m For_effects r sl a tmps) ->
+      (forall ge e le cp m, tr_top ge e le cp m For_effects r sl a tmps) ->
       tr_expr_stmt r (makeseq sl).
 
 Inductive tr_if: Csyntax.expr -> statement -> statement -> statement -> Prop :=
   | tr_if_intro: forall r s1 s2 sl a tmps,
-      (forall ge e le m, tr_top ge e le m For_val r sl a tmps) ->
+      (forall ge e le cp m, tr_top ge e le cp m For_val r sl a tmps) ->
       tr_if r s1 s2 (makeseq (sl ++ makeif a s1 s2 :: nil)).
 
 Inductive tr_stmt: Csyntax.statement -> statement -> Prop :=
@@ -1018,7 +1021,7 @@ Lemma transl_expr_meets_spec:
    forall r dst g sl a g' I,
    transl_expr dst r g = Res (sl, a) g' I ->
    dest_below dst g ->
-   exists tmps, forall ge e le m, tr_top ge e le m dst r sl a tmps.
+   exists tmps, forall ge e le cp m, tr_top ge e le cp m dst r sl a tmps.
 Proof.
   intros. exploit (proj1 transl_meets_spec); eauto. intros [tmps [A B]].
   exists (add_dest dst tmps); intros. apply tr_top_base. auto.
